

MATH 462 LECTURE NOTES: FEATURE REGRESSION

ADAM M. OBERMAN

The formulas above looks complicated at first glance. However, there is a geometrical interpretation in terms of projection. https://en.wikipedia.org/wiki/Projection_matrix

1. VECTOR DATASET NOTATION

Here we want to emphasize the fact that feature vectors are functions of the data.

So let x be a datapoint in an abstract data domain \mathcal{X} . In particular, we do not think of X as being a vectors space, since, for generic data, we do not have a notion of $x_1 + cx_2$.

We write a dataset

$$S_m = \{(x_1, y_1), \dots, (x_m, y_m)\}$$

in matrix form as

$$X = \begin{bmatrix} x_1 \\ x_2 \\ \vdots \\ x_m \end{bmatrix}, \quad X \in \mathcal{X}^{m \times 1}$$

and

$$Y = \begin{bmatrix} y_1 \\ y_2 \\ \vdots \\ y_m \end{bmatrix}, \quad Y \in \mathbb{R}^{m \times 1}$$

However, we assume that we have vector features, $f : \mathcal{X} \rightarrow \mathbb{R}^d$ written as a column vector,

$$f(x) = \begin{bmatrix} f^1(x) \\ \vdots \\ f^d(x) \end{bmatrix}$$

so that

$$f(x)^\top = [f^1(x), \dots, f^d(x)], \quad f(x) \in \mathbb{R}^{d \times 1}$$

is a row vector.

Note: since x is a column vector, the function $f(x) = x$ is also column vector, so we can think of a *vector-valued function as a vector of functions*.

1.1. Data Matrix. We are going to define, following the convention in [DFO20, Chapter 9] *Convention*. Note, if data/features are a column vector, then a matrix of data/features needs to be $m \times d$

Define

$$F = f(X)^\top = \begin{bmatrix} f(x_1)^\top \\ \vdots \\ f(x_m)^\top \end{bmatrix} = \begin{bmatrix} f^1(x_1) & \cdots & f^d(x_1) \\ \vdots & & \vdots \\ f^1(x_m) & \cdots & f^d(x_m) \end{bmatrix}, \quad F \in \mathbb{R}^{m \times d}$$

Thus we also have

$$F^\top = f(X) = \begin{bmatrix} f^1(x_1) & \cdots & f^1(x_m) \\ \vdots & & \vdots \\ f^d(x_1) & \cdots & f^d(x_m) \end{bmatrix}, \quad F \in \mathbb{R}^{d \times m}$$

Let $w \in \mathbb{R}^d$ be a column vector,

$$w = \begin{bmatrix} w_1 \\ \vdots \\ \vdots \\ w_d \end{bmatrix}$$

Then, we can write,

$$h(x) = f(x)^\top w$$

Linear functions of the features

$$\mathcal{H} = \{h : x \rightarrow \mathbb{R} \mid h(x) = f(x)^\top w, w \in \mathbb{R}^d\}$$

Write, in vector notation

$$\begin{aligned} H &= h(X) = Fw \\ E &= H - Y \end{aligned}$$

The mean squared loss

$$L(h, S) = \frac{1}{m} \sum_{i=1}^m (h(x_i) - y_i)^2$$

Can be written in vector notation as

$$L(h, S) = E^\top E = \|H - Y\|_2^2 = \|Fw - Y\|_2^2$$

Using the linear functions, we express the loss as a function of w ,

$$(1) \quad L(w) = \frac{1}{m} \sum_{i=1}^m (f(x_i) \cdot w - y_i)^2$$

1.2. Gradients and Jacobians. For a scalar function $h(x)$, we make $\nabla_x h$ a row vector. This way the jacobian of a vector valued function f is a matrix, where each row is $\nabla_x f^i$

Definition 1.1 (Jacobian). The collection of all first-order partial derivatives of a vector-valued function $f : \mathbb{R}^n \rightarrow \mathbb{R}^d$ is called the Jacobian. The Jacobian \mathbf{J} is an $d \times n$ matrix, which we define

and arrange as follows:

$$\mathbf{J} = \nabla_{\mathbf{x}} \mathbf{f} = \frac{d\mathbf{f}(\mathbf{x})}{d\mathbf{x}} = \left[\frac{\partial \mathbf{f}(\mathbf{x})}{\partial x_1} \quad \dots \quad \frac{\partial \mathbf{f}(\mathbf{x})}{\partial x_n} \right]$$

$$\mathbf{J} = \begin{bmatrix} \frac{\partial f_1(\mathbf{x})}{\partial x_1} & \dots & \frac{\partial f_1(\mathbf{x})}{\partial x_n} \\ \vdots & & \vdots \\ \frac{\partial f_d(\mathbf{x})}{\partial x_1} & \dots & \frac{\partial f_d(\mathbf{x})}{\partial x_n} \end{bmatrix},$$

where

$$\mathbf{x} = \begin{bmatrix} x_1 \\ \vdots \\ x_n \end{bmatrix},$$

so that

$$J(i, j) = \frac{\partial f_i}{\partial x_j}.$$

As a special case of (5.58), a function $f : \mathbb{R}^n \rightarrow \mathbb{R}^1$, which maps a vector $\mathbf{x} \in \mathbb{R}^n$ onto a scalar (e.g., $f(\mathbf{x}) = \sum_{i=1}^n a_i x_i$), possesses a Jacobian that is a row vector (matrix of dimension $1 \times n$).

Example 1.2. Let $f(x) = a^\top x = x^\top a$ be linear. Note, x is a column vector, and a is a column vector. Then $\nabla_x f(x) = a^\top$ is a row vector. However, we define $\nabla_a f(x) = x$ to be a *column* vector, to be consistent with the notion that a vector of functions is a column vector. Thus

$f(x) = a^\top x$	scalar function
$\nabla_x f(x) = a^\top$	row vector (gradient in x)
$\nabla_a f(x) = x$	column vector (vector of functions)

Example 1.3. Now when w is the variable, and x is a parameter, let $L(w, x) = (w^\top x - y)^2/2$. Then

$L(w, x) = (w^\top x - y)^2/2$	scalar function of w
$\nabla_w L = (w^\top x - y)x^\top$	row vector (gradient in w)
$\nabla_x L = (w^\top x - y)w$	column vector (vector of functions of w)

1.3. Feature regression minimizer. Going back to the vector notation for the loss, (1),

$$L(w) = \frac{1}{m} \sum_{i=1}^m (f(x_i) \cdot w - y_i)^2$$

Taking a derivative

$$\frac{\partial L}{\partial w_j}(w) = \frac{1}{m} \sum_{i=1}^m (f(x_i) \cdot w - y_i) (2f^j(x_i))$$

Now for the gradient (which is a row vector),

$$\nabla_w L(w) = \frac{2}{m} \sum_{i=1}^m (f(x_i) \cdot w - y_i) f(x_i)^\top$$

in vector notation, this is

$$\frac{2}{m} E^T F^T = \frac{2}{m} F^T (Fw - Y)$$

Thus, in vector notation

$$\nabla_w L(w) = \frac{2}{m} F^T (Fw - Y)$$

So the minimizer satisfies the normal equation

$$(2) \quad F^T Fw = F^T Y$$

Which means

$$w = (F^T F)^{-1} F^T y$$

Then the function values are

$$h = Fw = F(F^T F)^{-1} F^T y$$

and for new function values,

$$h(x) = f(x) \cdot w = f(x) \cdot (F^T F)^{-1} F^T y$$

2. FUNCTIONAL NOTATION

2.1. Inner product of functions. Let H be a vector space of functions, with an inner product $(f, g) = (f, g)_H$.

We are now going to write the regression problem as a projection problem in function space.

Given $y \in H$, and given functions f_1, \dots, f_d , let

$$V = \text{span}\{f_1, \dots, f_d\}$$

Let

$$h = \text{Proj}_V(y) = \arg \min_{f \in V} \|f - y\|_H^2$$

Since h is the projection, for each basis element $f_i \in V$, we have

$$(h, f_i) = (y, f_i)$$

Write $h = \sum w_j f_j$. Then

$$\left(\sum w_i f_i, f_j \right) = (y, f_j), \quad \forall j$$

or

$$\sum_i w_i (f_i, f_j) = (y, f_j)$$

Define $M_{ij} = (f_i, f_j)$ and $b_j = (y, f_j)$. Then equation becomes

$$Mw = b$$

This makes more intuitive sense to me than the vector way.

If, instead, we find an orthonormal basis of V , say, e_1, \dots, e_d , then the equations become

$$\left(\sum w_i e_i, e_j \right) = (y, e_j), \quad \forall j$$

or

$$w_i = (y, e_i), \quad \forall i$$

Leading to the projection

$$h = \sum_i (y, e_i) e_i$$

2.2. **Analysis of the minimizer.** Define the vector space $V = V(X)$ to be m -dimensional vectors, regarded as functions

$$V = \{f : X \rightarrow \mathbb{R} \mid f_i = f(x_i)\}$$

Define an inner product on V by

$$(h, g)_X = \frac{1}{m} \sum_{i=1}^m g(x_i)h(x_i)$$

Then the normal equation can be interpreted as follows

$$(F^\top F)_{ij} = (f^i, f^j)_X, \quad (F^\top Y)_j = (y, f^j)_X$$

and

$$h(X) = w \cdot f(X)$$

is the projection of Y onto the span of F .

we also have the following result.

The error is orthogonal to the solution

Theorem 2.1. *Let Y be given as above. Let $H = Fw$ be the solution of the normal equation. Let $E = H - Y$ be the error. Then the error is orthogonal to the solution,*

$$(E, H)_X = 0$$

Proof. From the normal equation, (2)

$$F^\top (Fw - Y) = 0$$

multiply on the right by w^\top , to obtain

$$w^\top F^\top (Fw - Y) = 0$$

rewrite this as

$$(H, E) = 0$$

as desired. □

REFERENCES

[DF020] Marc Peter Deisenroth, A Aldo Faisal, and Cheng Soon Ong. *Mathematics for machine learning*. Cambridge University Press, 2020.